src/program_proof/wal/write_proof.v
@@ -315,14 +315,13 @@ Proof.
     destruct matches; lia.
 Qed.
 
-Lemma is_durable_append γ txns txns' installed_txn_id diskEnd_txn_id :
+Lemma is_durable_append γ cs txns txns' installed_txn_id diskEnd_txn_id :
   (diskEnd_txn_id < length txns)%nat ->
-  is_durable γ txns installed_txn_id diskEnd_txn_id -∗
-  is_durable γ (txns ++ txns') installed_txn_id diskEnd_txn_id.
+  is_durable γ cs txns installed_txn_id diskEnd_txn_id -∗
+  is_durable γ cs (txns ++ txns') installed_txn_id diskEnd_txn_id.
 Proof.
   intros Hbound.
   rewrite /is_durable; iNamed 1.
-  iExists _; iFrame.
   iPureIntro.
   rewrite /circ_matches_txns in Hcirc_matches |- *.
   rewrite -> subslice_app_1 by lia; auto.
